pulse/src/checker/Pulse.Soundness.STT.fsti
@@ -45,7 +45,7 @@ val stt_atomic_typing (#obs:R.term)
                       (_:RT.tot_typing f inames inames_tm)
                       (_:RT.tot_typing f pre vprop_tm)
                       (_:RT.tot_typing f post (post_type t))
-  : GTot (RT.tot_typing f (mk_stt_atomic_comp obs u t inames pre post) (RT.tm_type (u_max_two u)))
+  : GTot (RT.tot_typing f (mk_stt_atomic_comp obs u t inames pre post) (RT.tm_type (u_atomic_ghost u)))
 
 val stt_ghost_typing (#f:RT.fstar_env)//needs to bind stt
                      (#u:R.universe)
@@ -55,4 +55,4 @@ val stt_ghost_typing (#f:RT.fstar_env)//needs to bind stt
                      (_:RT.tot_typing f t (RT.tm_type u))
                      (_:RT.tot_typing f pre vprop_tm)
                      (_:RT.tot_typing f post (post_type t))
-  : GTot (RT.tot_typing f (mk_stt_ghost_comp u t pre post) (RT.tm_type (u_max_two u)))
+  : GTot (RT.tot_typing f (mk_stt_ghost_comp u t pre post) (RT.tm_type (u_atomic_ghost u)))
